Make methods static

Rope.dfy
@@ -1,16 +1,12 @@
-include "Utils.dfy"
-
 module Rope {
-    import Utils
-
-    class Node {
+    class Rope {
         ghost var Contents: string;
-        ghost var Repr: set<Node>;
+        ghost var Repr: set<Rope>;
 
         var data: string;
         var weight: nat;
-        var left: Node?;
-        var right: Node?;
+        var left: Rope?;
+        var right: Rope?;
 
         ghost predicate Valid() 
             reads this, Repr
@@ -49,7 +45,7 @@ module Rope {
                 data == "") 
         }
 
-        static lemma contentSizeGtZero(n: Node)
+        static lemma contentSizeGtZero(n: Rope)
             requires n.Valid()
             ensures |n.Contents| > 0
             decreases n.Repr
@@ -76,12 +72,12 @@ module Rope {
             Repr := {this};
         }   
 
-        predicate isTerminal(n: Node)
+        predicate isTerminal(n: Rope)
             reads n, n.left, n.right
         { n.left == null && n.right == null }
 
         // constructor for creating a non-terminal node
-        constructor NonTerminal(nLeft: Node, nRight: Node)
+        constructor NonTerminal(nLeft: Rope, nRight: Rope)
             requires nLeft.Valid() && nRight.Valid() && nLeft.Repr !! nRight.Repr
             ensures Valid() && left == nLeft && right == nRight && fresh(Repr - nLeft.Repr - nRight.Repr)
         { 
@@ -91,7 +87,7 @@ module Rope {
 
             var nTemp := nLeft;
             var w := 0;
-            ghost var nodesTraversed : set<Node> := {};
+            ghost var nodesTraversed : set<Rope> := {};
 
             while (nTemp.right != null)
                 invariant nTemp != null
@@ -123,7 +119,7 @@ module Rope {
             Repr := {this} + nLeft.Repr + nRight.Repr;
         }   
 
-        method getCharAtIndex(index: nat) returns (nTemp: Node, i: nat, c: char)
+        method getCharAtIndex(index: nat) returns (nTemp: Rope, i: nat, c: char)
             requires Valid() && 0 <= index < |Contents|
             ensures c == Contents[index]
             ensures 0 <= i < |nTemp.data|
@@ -148,7 +144,6 @@ module Rope {
             // Have reached the terminal node with index i
             c := nTemp.data[i];
         }
-
 
         method report(i: nat, j: nat) returns (s: string)
             requires 0 <= i <= j <= |this.Contents|
@@ -183,114 +178,112 @@ module Rope {
             }
         }
 
-    }
-    // End of Node Class
-
-
-    method concat(n1: Node?, n2: Node?) returns (n: Node?) 
-        requires (n1 != null) ==> n1.Valid()
-        requires (n2 != null) ==> n2.Valid()
-        requires (n1 != null && n2 != null) ==> (n1.Repr !! n2.Repr)
-        ensures (n1 != null || n2 != null) ==> n != null && n.Valid()
-        ensures (n1 == null && n2 == null) ==> n == null
-        ensures (n1 == null && n2 != null) ==> n == n2 && n != null && n.Valid() && n.Contents == n2.Contents
-        ensures (n1 != null && n2 == null) ==> n == n1 && n != null && n.Valid() && n.Contents == n1.Contents
-        ensures (n1 != null && n2 != null) ==> (n != null && n.Valid() && n.left == n1 && n.right == n2 && 
-                                                n.Contents == n1.Contents + n2.Contents && fresh(n.Repr - n1.Repr - n2.Repr))
-    {
-        if (n1 == null) {
-            n := n2;
-        } else if (n2 == null) {
-            n := n1;
-        } else {
-            n := new Node.NonTerminal(n1, n2);
-        } 
-    } 
-
-
-    /**
-        Dafny needs help to guess that in our definition, every rope must
-        have non-empty Contents, otherwise it is represented by [null].
-
-        The lemma contentSizeGtZero(n) is thus important to prove the
-        postcondition of this method, in the two places where the lemma is
-        invoked.
-     */
-    method split(n: Node, index: nat) returns (n1: Node?, n2: Node?) 
-        requires n.Valid() && 0 <= index <= |n.Contents|
-        ensures index == 0 ==> (n1 == null && n2 != null && n2.Valid() && n2.Contents == n.Contents && fresh(n2.Repr - n.Repr))
-        ensures index == |n.Contents| ==> (n2 == null && n1 != null && n1.Valid() && n1.Contents == n.Contents && fresh(n1.Repr - n.Repr))
-        ensures 0 < index < |n.Contents| ==> (n1 != null && n1.Valid() && n2 != null && n2.Valid() && 
-                                                n1.Contents == n.Contents[..index] && n2.Contents == n.Contents[index..] &&
-                                                n1.Repr !! n2.Repr && fresh(n1.Repr - n.Repr) && fresh(n2.Repr - n.Repr))
-        decreases n.Repr
-    {
-        if (index == 0) {
-            n1 := null;
-            n2 := n;
-            Node.contentSizeGtZero(n);
-            // assert index != |n.Contents|;
-        } else if (index < n.weight) {
-            if (n.left != null) {
-                var s1, s2 := split(n.left, index);
-                n1 := s1;
-                n2 := concat(s2, n.right);
+        static method concat(n1: Rope?, n2: Rope?) returns (n: Rope?) 
+            requires (n1 != null) ==> n1.Valid()
+            requires (n2 != null) ==> n2.Valid()
+            requires (n1 != null && n2 != null) ==> (n1.Repr !! n2.Repr)
+            ensures (n1 != null || n2 != null) ==> n != null && n.Valid()
+            ensures (n1 == null && n2 == null) ==> n == null
+            ensures (n1 == null && n2 != null) ==> n == n2 && n != null && n.Valid() && n.Contents == n2.Contents
+            ensures (n1 != null && n2 == null) ==> n == n1 && n != null && n.Valid() && n.Contents == n1.Contents
+            ensures (n1 != null && n2 != null) ==> (n != null && n.Valid() && n.left == n1 && n.right == n2 && 
+                                                    n.Contents == n1.Contents + n2.Contents && fresh(n.Repr - n1.Repr - n2.Repr))
+        {
+            if (n1 == null) {
+                n := n2;
+            } else if (n2 == null) {
+                n := n1;
             } else {
-                // terminal node
-                if (index == 0) {
-                    n1 := null;
-                    n2 := n;
+                n := new Rope.NonTerminal(n1, n2);
+            } 
+        } 
+
+
+        /**
+            Dafny needs help to guess that in our definition, every rope must
+            have non-empty Contents, otherwise it is represented by [null].
+
+            The lemma contentSizeGtZero(n) is thus important to prove the
+            postcondition of this method, in the two places where the lemma is
+            invoked.
+        */
+        static method split(n: Rope, index: nat) returns (n1: Rope?, n2: Rope?) 
+            requires n.Valid() && 0 <= index <= |n.Contents|
+            ensures index == 0 ==> (n1 == null && n2 != null && n2.Valid() && n2.Contents == n.Contents && fresh(n2.Repr - n.Repr))
+            ensures index == |n.Contents| ==> (n2 == null && n1 != null && n1.Valid() && n1.Contents == n.Contents && fresh(n1.Repr - n.Repr))
+            ensures 0 < index < |n.Contents| ==> (n1 != null && n1.Valid() && n2 != null && n2.Valid() && 
+                                                    n1.Contents == n.Contents[..index] && n2.Contents == n.Contents[index..] &&
+                                                    n1.Repr !! n2.Repr && fresh(n1.Repr - n.Repr) && fresh(n2.Repr - n.Repr))
+            decreases n.Repr
+        {
+            if (index == 0) {
+                n1 := null;
+                n2 := n;
+                Rope.contentSizeGtZero(n);
+                // assert index != |n.Contents|;
+            } else if (index < n.weight) {
+                if (n.left != null) {
+                    var s1, s2 := split(n.left, index);
+                    n1 := s1;
+                    n2 := concat(s2, n.right);
                 } else {
-                    n1 := new Node.Terminal(n.data[..index]);
-                    n2 := new Node.Terminal(n.data[index..]);
+                    // terminal node
+                    if (index == 0) {
+                        n1 := null;
+                        n2 := n;
+                    } else {
+                        n1 := new Rope.Terminal(n.data[..index]);
+                        n2 := new Rope.Terminal(n.data[index..]);
+                    }
+                }
+            } else if (index > n.weight) {
+                var s1, s2 := split(n.right, index - n.weight);
+                n1 := concat(n.left, s1);
+                n2 := s2;
+            } else {
+                // since [n.weight == index != 0], it means that [n] cannot be a
+                // non-terminal node with [left == null].
+                if (n.left != null && n.right == null) {
+                    n1 := n.left;
+                    n2 := null;
+                } else if (n.left != null && n.right != null) {
+                    n.contentSizeGtZero(n.right);
+                    // assert index != |n.Contents|;
+                    n1 := n.left;
+                    n2 := n.right;
+                } else {
+                    assert n.left == null && n.right == null;
+                    n1 := n;
+                    n2 := null;
                 }
             }
-        } else if (index > n.weight) {
-            var s1, s2 := split(n.right, index - n.weight);
-            n1 := concat(n.left, s1);
-            n2 := s2;
-        } else {
-            // since [n.weight == index != 0], it means that [n] cannot be a
-            // non-terminal node with [left == null].
-            if (n.left != null && n.right == null) {
-                n1 := n.left;
-                n2 := null;
-            } else if (n.left != null && n.right != null) {
-                n.contentSizeGtZero(n.right);
-                // assert index != |n.Contents|;
-                n1 := n.left;
-                n2 := n.right;
-            } else {
-                assert n.left == null && n.right == null;
-                n1 := n;
-                n2 := null;
-            }
         }
-    }
 
-    method insert(n1: Node, n2: Node, index: nat) returns (n: Node)
-        requires n1.Valid() && n2.Valid() && n1.Repr !! n2.Repr
-        requires 0 <= index < |n1.Contents|
-        ensures n.Valid() && n.Contents == n1.Contents[..index] + n2.Contents + n1.Contents[index..] && fresh(n.Repr - n1.Repr - n2.Repr)
-    {
-        var n1BeforeIndex, n1AfterIndex := split(n1, index);
-        var firstPart := concat(n1BeforeIndex, n2);
-        n := concat(firstPart, n1AfterIndex);
-    }
+        static method insert(n1: Rope, n2: Rope, index: nat) returns (n: Rope)
+            requires n1.Valid() && n2.Valid() && n1.Repr !! n2.Repr
+            requires 0 <= index < |n1.Contents|
+            ensures n.Valid() && n.Contents == n1.Contents[..index] + n2.Contents + n1.Contents[index..] && fresh(n.Repr - n1.Repr - n2.Repr)
+        {
+            var n1BeforeIndex, n1AfterIndex := split(n1, index);
+            var firstPart := concat(n1BeforeIndex, n2);
+            n := concat(firstPart, n1AfterIndex);
+        }
 
-    method delete(n: Node, i: nat, j: nat) returns (m: Node?)
-        requires n.Valid()
-        requires 0 <= i < j <= |n.Contents|
-        ensures (i == 0 && j == |n.Contents|) <==> m == null
-        ensures m != null ==>
-            m.Valid() &&
-            m.Contents == n.Contents[..i] + n.Contents[j..] &&
-            fresh(m.Repr - n.Repr)
-        
-    {
-        var l1, l2 := split(n, i);
-        var r1, r2 := split(l2, j - i);
-        m := concat(l1, r2);
+        static method delete(n: Rope, i: nat, j: nat) returns (m: Rope?)
+            requires n.Valid()
+            requires 0 <= i < j <= |n.Contents|
+            ensures (i == 0 && j == |n.Contents|) <==> m == null
+            ensures m != null ==>
+                m.Valid() &&
+                m.Contents == n.Contents[..i] + n.Contents[j..] &&
+                fresh(m.Repr - n.Repr)
+        {
+            var l1, l2 := split(n, i);
+            var r1, r2 := split(l2, j - i);
+            m := concat(l1, r2);
+        }
+
     }
+    // End of Rope Class
 }
 // End of Rope Module
