Test.dfy
@@ -3,32 +3,31 @@ import opened Rope
 
 method test()
 {
-    var n := new Node.Terminal("Hello ");
+    var n := new Rope.Terminal("Hello ");
     assert n.Valid() && n.weight == 6 && n.data == "Hello " && n.Repr == {n} && n.Contents == "Hello ";
-    var n1 := new Node.Terminal("my ");
+    var n1 := new Rope.Terminal("my ");
     assert n1.Valid() && n1.Repr !! n.Repr;
-    var n2 := concat(n, n1);
+    var n2 := Rope.concat(n, n1);
     assert n2.Contents == "Hello my " && n2.left == n && n2.right == n1 && n2.weight == |n.Contents|;
-    var n3 := new Node.Terminal("na");
+    var n3 := new Rope.Terminal("na");
     assert n3.weight == 2;
-    var n4 := new Node.Terminal("me i");
-    var n5 := concat(n3, n4);
+    var n4 := new Rope.Terminal("me i");
+    var n5 := Rope.concat(n3, n4);
     assert n5.weight == 2;
-    var n6 := new Node.Terminal("s");
-    var n7 := new Node.Terminal(" Simon");
-    var n8 := concat(n6, n7);
-    var n9 := concat(n5, n8);
-    var B := concat(n2, n9);
+    var n6 := new Rope.Terminal("s");
+    var n7 := new Rope.Terminal(" Simon");
+    var n8 := Rope.concat(n6, n7);
+    var n9 := Rope.concat(n5, n8);
+    var B := Rope.concat(n2, n9);
     assert B.weight == 9 && B.Contents == "Hello my name is Simon";
-    var AHopeful := concat(B, null);
+    var AHopeful := Rope.concat(B, null);
     assert AHopeful == B;
     assert AHopeful.weight == 9;
     assert AHopeful.Contents == B.Contents;
 
-    var foo := delete(AHopeful, 0, 1);
+    var foo := Rope.delete(AHopeful, 0, 1);
     assert foo.Contents == "ello my name is Simon";
     var s := foo.report(1,3);
     assert s == "ll";
     print s;
 }
-
